Obc/ObcSemantics.v
@@ -70,8 +70,7 @@ Module Type OBCSEMANTICS
       madd_mem x v menv = menv' ->
       stmt_eval prog menv env (AssignSt x e) (menv', env)
   | Icall: forall prog menv env es vs clsid o f ys menv' env' omenv omenv' rvs,
-      omenv = match mfind_inst o menv with None => hempty
-                                         | Some om => om end ->
+      omenv = match mfind_inst o menv with None => hempty | Some om => om end ->
       Forall2 (exp_eval menv env) es vs ->
       stmt_call_eval prog omenv clsid f vs omenv' rvs ->
       madd_obj o omenv' menv = menv' ->
